
\documentclass{article}
%%%%%%%%%%%%%%%%%%%%%%%%%%%%%%%%%%%%%%%%%%%%%%%%%%%%%%%%%%%%%%%%%%%%%%%%%%%%%%%%%%%%%%%%%%%%%%%%%%%%%%%%%%%%%%%%%%%%%%%%%%%%
\usepackage{graphicx}
\usepackage{amsmath}

%TCIDATA{OutputFilter=LATEX.DLL}
%TCIDATA{Created=Thu Jan 22 22:41:22 2004}
%TCIDATA{LastRevised=Fri Jan 23 00:41:04 2004}
%TCIDATA{<META NAME="GraphicsSave" CONTENT="32">}
%TCIDATA{<META NAME="DocumentShell" CONTENT="General\Blank Document">}
%TCIDATA{CSTFile=LaTeX article (bright).cst}
%TCIDATA{MapleDefs=
%$d=(\frac{1}{\sqrt{2}})(-\frac{5}{8}-\frac{1}{8})=-\frac{3}{8}\sqrt{2}$
%$c=(\frac{1}{\sqrt{2}})(-\frac{5}{8}+\frac{1}{8})=-\frac{1}{4}\sqrt{2}$
%$b=(\frac{1}{\sqrt{2}})(\frac{7}{16}-\frac{5}{16})=\frac{1}{16}\sqrt{2}$
%$a=(\frac{1}{\sqrt{2}})(\frac{7}{16}+\frac{5}{16})=\frac{3}{8}\sqrt{2}$
%$z=\frac{1}{2}$
%$y=\frac{1}{2}$
%$x=\frac{1}{2}$
%$w=0$
%}


\newtheorem{theorem}{Theorem}
\newtheorem{acknowledgement}[theorem]{Acknowledgement}
\newtheorem{algorithm}[theorem]{Algorithm}
\newtheorem{axiom}[theorem]{Axiom}
\newtheorem{case}[theorem]{Case}
\newtheorem{claim}[theorem]{Claim}
\newtheorem{conclusion}[theorem]{Conclusion}
\newtheorem{condition}[theorem]{Condition}
\newtheorem{conjecture}[theorem]{Conjecture}
\newtheorem{corollary}[theorem]{Corollary}
\newtheorem{criterion}[theorem]{Criterion}
\newtheorem{definition}[theorem]{Definition}
\newtheorem{example}[theorem]{Example}
\newtheorem{exercise}[theorem]{Exercise}
\newtheorem{lemma}[theorem]{Lemma}
\newtheorem{notation}[theorem]{Notation}
\newtheorem{problem}[theorem]{Problem}
\newtheorem{proposition}[theorem]{Proposition}
\newtheorem{remark}[theorem]{Remark}
\newtheorem{solution}[theorem]{Solution}
\newtheorem{summary}[theorem]{Summary}
\newenvironment{proof}[1][Proof]{\textbf{#1.} }{\ \rule{0.5em}{0.5em}}
%\input{tcilatex}

\begin{document}


$
\begin{array}{cc}
\frac{1}{2} & \frac{1}{2} \\ 
0 & \frac{1}{2}
\end{array}
\cdot 
\begin{array}{cc}
\frac{1}{2} & \frac{1}{2} \\ 
0 & \frac{1}{2}
\end{array}
=\allowbreak 
\begin{array}{cc}
\frac{1}{2} & \frac{1}{2} \\ 
0 & \frac{1}{2}
\end{array}
^{2}=\allowbreak 
\begin{array}{cc}
\frac{1}{4} & \frac{1}{2} \\ 
0 & \frac{1}{4}
\end{array}
$

$(\frac{1}{\sqrt{2}})
\begin{array}{cc}
1 & 0 \\ 
\frac{1}{2} & 0
\end{array}
$

$(1-\frac{1}{2})(\frac{1}{\sqrt{2}})(\frac{1}{\sqrt{2}})=\allowbreak \frac{1%
}{4}$

$(1+\frac{1}{2})(\frac{1}{\sqrt{2}})(\frac{1}{\sqrt{2}})=\allowbreak \frac{3%
}{4}$

$
\begin{array}{cc}
\frac{3}{4} & \frac{1}{2} \\ 
\frac{1}{4} & -\frac{1}{2}
\end{array}
\cdot 
\begin{array}{cc}
\frac{3}{4} & \frac{1}{2} \\ 
\frac{1}{4} & -\frac{1}{2}
\end{array}
=\allowbreak 
\begin{array}{cc}
\frac{3}{4} & \frac{1}{2} \\ 
\frac{1}{4} & -\frac{1}{2}
\end{array}
^{2}=\allowbreak 
\begin{array}{cc}
\frac{11}{16} & \frac{1}{8} \\ 
\frac{1}{16} & \frac{3}{8}
\end{array}
$

$a=(\frac{1}{\sqrt{2}})(\frac{7}{16}+\frac{5}{16})=\allowbreak \frac{3}{8}%
\sqrt{2}$

$b=(\frac{1}{\sqrt{2}})(\frac{7}{16}-\frac{5}{16})=\allowbreak \frac{1}{16}%
\sqrt{2}$

$c=(\frac{1}{\sqrt{2}})(-\frac{5}{8}+\frac{1}{8})=\allowbreak -\frac{1}{4}%
\sqrt{2}$

$d=(\frac{1}{\sqrt{2}})(-\frac{5}{8}-\frac{1}{8})=\allowbreak -\frac{3}{8}%
\sqrt{2}$

\bigskip 

$(\frac{\sqrt{2}}{2})(b-d)=\allowbreak \frac{7}{16}=\frac{7}{16}$

$(\frac{\sqrt{2}}{2})(b+d)=\allowbreak -\frac{5}{16}=-\frac{5}{16}$

$\frac{1}{\sqrt{2}}(a-c)=\allowbreak \frac{5}{8}=\frac{5}{8}$

$\frac{1}{\sqrt{2}}(a+c)=\allowbreak \frac{1}{8}=\frac{1}{8}$

$\frac{1}{2}
\begin{array}{cc}
x+y+w+z & x-y+w-z \\ 
x+y-w-z & x-y-w+z
\end{array}
\cdot \frac{1}{2}
\begin{array}{cc}
x+y+w+z & x-y+w-z \\ 
x+y-w-z & x-y-w+z
\end{array}
=
\begin{array}{cc}
\frac{1}{2}x^{2}+\frac{1}{2}xy+\frac{1}{2}xw+yw+\frac{1}{2}yz+\frac{1}{2}wz+%
\frac{1}{2}z^{2} & \frac{1}{2}x^{2}+\frac{1}{2}xw-\frac{1}{2}yz-\frac{1}{2}%
z^{2}-\frac{1}{2}xy+\frac{1}{2}wz \\ 
\frac{1}{2}x^{2}+\frac{1}{2}xy-\frac{1}{2}wz-\frac{1}{2}z^{2}-\frac{1}{2}xw+%
\frac{1}{2}yz & \frac{1}{2}x^{2}+yw+\frac{1}{2}z^{2}-\frac{1}{2}xy-\frac{1}{2%
}xw-\frac{1}{2}yz-\frac{1}{2}wz
\end{array}
\allowbreak $

$\frac{(\frac{1}{2}x^{2}+\frac{1}{2}xy+\frac{1}{2}xw+yw+\frac{1}{2}yz+\frac{1%
}{2}wz+\frac{1}{2}z^{2})-(\frac{1}{2}x^{2}+\frac{1}{2}xy-\frac{1}{2}wz-\frac{%
1}{2}z^{2}-\frac{1}{2}xw+\frac{1}{2}yz)}{\sqrt{2}}=\allowbreak \frac{1}{2}%
\left( xw+yw+wz+z^{2}\right) \sqrt{2}$

$\frac{(\frac{1}{2}x^{2}+\frac{1}{2}xy+\frac{1}{2}xw+yw+\frac{1}{2}yz+\frac{1%
}{2}wz+\frac{1}{2}z^{2})+(\frac{1}{2}x^{2}+\frac{1}{2}xy-\frac{1}{2}wz-\frac{%
1}{2}z^{2}-\frac{1}{2}xw+\frac{1}{2}yz)}{\sqrt{2}}=\allowbreak \frac{1}{2}%
\left( x^{2}+xy+yw+yz\right) \sqrt{2}$

$\frac{(\frac{1}{2}x^{2}+\frac{1}{2}xw-\frac{1}{2}yz-\frac{1}{2}z^{2}-\frac{1%
}{2}xy+\frac{1}{2}wz)-(\frac{1}{2}x^{2}+yw+\frac{1}{2}z^{2}-\frac{1}{2}xy-%
\frac{1}{2}xw-\frac{1}{2}yz-\frac{1}{2}wz)}{\sqrt{2}}=\allowbreak \frac{1}{2}%
\left( xw-z^{2}+wz-yw\right) \sqrt{2}$

$\frac{(\frac{1}{2}x^{2}+\frac{1}{2}xw-\frac{1}{2}yz-\frac{1}{2}z^{2}-\frac{1%
}{2}xy+\frac{1}{2}wz)+(\frac{1}{2}x^{2}+yw+\frac{1}{2}z^{2}-\frac{1}{2}xy-%
\frac{1}{2}xw-\frac{1}{2}yz-\frac{1}{2}wz)}{\sqrt{2}}\ =\allowbreak \frac{1}{%
2}\left( x^{2}-yz-xy+yw\right) \sqrt{2}$

$\frac{(\frac{1}{2}\left( xw+yw+wz+z^{2}\right) \sqrt{2})-(\frac{1}{2}\left(
xw-z^{2}+wz-yw\right) \sqrt{2})}{\sqrt{2}}=\allowbreak yw+z^{2}=\allowbreak 
\frac{1}{4}$

$\frac{(\frac{1}{2}\left( xw+yw+wz+z^{2}\right) \sqrt{2})+(\frac{1}{2}\left(
xw-z^{2}+wz-yw\right) \sqrt{2})}{\sqrt{2}}=\allowbreak w\left( x+z\right)
=\allowbreak 0$

$\frac{(\allowbreak \frac{1}{2}\left( x^{2}+xy+yw+yz\right) \sqrt{2})-(\frac{%
1}{2}\left( xw-z^{2}+wz-yw\right) \sqrt{2})}{\sqrt{2}}=\allowbreak \frac{1}{2%
}x^{2}+\frac{1}{2}xy+yw+\frac{1}{2}yz-\frac{1}{2}xw+\frac{1}{2}z^{2}-\frac{1%
}{2}wz=\allowbreak \frac{1}{2}$

$\frac{(\allowbreak \frac{1}{2}\left( x^{2}+xy+yw+yz\right) \sqrt{2})+(\frac{%
1}{2}\left( xw-z^{2}+wz-yw\right) \sqrt{2})}{\sqrt{2}}=\allowbreak \frac{1}{2%
}x^{2}+\frac{1}{2}xy+\frac{1}{2}yz+\frac{1}{2}xw-\frac{1}{2}z^{2}+\frac{1}{2}%
wz=\allowbreak \frac{1}{4}$

$x=\frac{1}{2}$

$y=\frac{1}{2}$

$z=\frac{1}{2}$

$w=0$

$
\begin{array}{cc}
\frac{1}{2}x^{2}+\frac{1}{2}xy+\frac{1}{2}xw+yw+\frac{1}{2}yz+\frac{1}{2}wz+%
\frac{1}{2}z^{2} & \frac{1}{2}x^{2}+\frac{1}{2}xw-\frac{1}{2}yz-\frac{1}{2}%
z^{2}-\frac{1}{2}xy+\frac{1}{2}wz \\ 
\frac{1}{2}x^{2}+\frac{1}{2}xy-\frac{1}{2}wz-\frac{1}{2}z^{2}-\frac{1}{2}xw+%
\frac{1}{2}yz & \frac{1}{2}x^{2}+yw+\frac{1}{2}z^{2}-\frac{1}{2}xy-\frac{1}{2%
}xw-\frac{1}{2}yz-\frac{1}{2}wz
\end{array}
\allowbreak =\allowbreak 
\begin{array}{cc}
\frac{1}{2} & -\frac{1}{4} \\ 
\frac{1}{4} & 0
\end{array}
$

$\frac{1}{2}
\begin{array}{cc}
x+y+w+z & x-y+w-z \\ 
x+y-w-z & x-y-w+z
\end{array}
=\allowbreak 
\begin{array}{cc}
\frac{3}{4} & -\frac{1}{4} \\ 
\frac{1}{4} & \frac{1}{4}
\end{array}
$

\bigskip 

\end{document}
